<?xml version="1.0" encoding="UTF-8"?>
<rdf:RDF
   xmlns:dc="http://purl.org/dc/terms/"
   xmlns:owl="http://www.w3.org/2002/07/owl#"
   xmlns:rdf="http://www.w3.org/1999/02/22-rdf-syntax-ns#"
   xmlns:rdfs="http://www.w3.org/2000/01/rdf-schema#"
   xmlns:skos="http://www.w3.org/2004/02/skos/core#"
   xmlns:vs="http://www.w3.org/2003/06/sw-vocab-status/ns#"
>
  <rdf:Description rdf:about="http://ns.science.ai/.#Unspecified">
    <owl:disjointWith rdf:resource="http://ns.science.ai/#Reference"/>
    <owl:disjointWith rdf:resource="http://ns.science.ai/#Discussion"/>
    <rdfs:isDefinedBy rdf:resource="https://ns.science.ai/"/>
    <vs:term_status>testing</vs:term_status>
    <owl:disjointWith rdf:resource="http://ns.science.ai/#Conclusion"/>
    <rdfs:label>Unspecified</rdfs:label>
    <owl:disjointWith rdf:resource="http://ns.science.ai/#Image"/>
    <owl:disjointWith rdf:resource="http://ns.science.ai/#Funding"/>
    <owl:disjointWith rdf:resource="http://ns.science.ai/#SupportingInformation"/>
    <owl:disjointWith rdf:resource="http://ns.science.ai/#ReferenceList"/>
    <owl:disjointWith rdf:resource="http://ns.science.ai/#Audio"/>
    <rdf:type rdf:resource="http://www.w3.org/2000/01/rdf-schema#Class"/>
    <owl:disjointWith rdf:resource="http://ns.science.ai/#Acknowledgements"/>
    <owl:disjointWith rdf:resource="http://ns.science.ai/#Abstract"/>
    <owl:disjointWith rdf:resource="http://ns.science.ai/#Affiliations"/>
    <owl:disjointWith rdf:resource="http://ns.science.ai/#MaterialsAndMethods"/>
    <owl:disjointWith rdf:resource="http://ns.science.ai/#Formula"/>
    <owl:disjointWith rdf:resource="http://ns.science.ai/#Introduction"/>
    <owl:disjointWith rdf:resource="http://ns.science.ai/#Results"/>
    <owl:disjointWith rdf:resource="http://ns.science.ai/#Disclosure"/>
    <owl:disjointWith rdf:resource="http://ns.science.ai/#Table"/>
    <rdfs:comment>A section that is unknown or otherwise unspecified.</rdfs:comment>
    <owl:disjointWith rdf:resource="http://ns.science.ai/#Authors"/>
    <owl:disjointWith rdf:resource="http://ns.science.ai/#Contributors"/>
    <owl:disjointWith rdf:resource="http://ns.science.ai/#Video"/>
  </rdf:Description>
  <rdf:Description rdf:about="http://ns.science.ai/.#RdfaConversionAction">
    <rdfs:label>RDFaConversionAction</rdfs:label>
    <skos:altLabel>RDFa Conversion Action</skos:altLabel>
    <rdfs:comment>The act of converting an object to RDFa (HTML web document with rich structured data markup).</rdfs:comment>
    <rdfs:isDefinedBy rdf:resource="https://ns.science.ai/"/>
    <vs:term_status>testing</vs:term_status>
    <rdfs:subClassOf rdf:resource="http://schema.org/Action"/>
    <rdf:type rdf:resource="http://www.w3.org/2000/01/rdf-schema#Class"/>
  </rdf:Description>
  <rdf:Description rdf:about="http://ns.science.ai/.#roleOffer">
    <skos:altLabel>role offer</skos:altLabel>
    <rdfs:isDefinedBy rdf:resource="https://ns.science.ai/"/>
    <vs:term_status>testing</vs:term_status>
    <rdfs:label>roleOffer</rdfs:label>
    <rdfs:domain rdf:resource="http://ns.science.ai/#SponsorRole"/>
    <rdfs:comment>An offer made by the role's sponsor.</rdfs:comment>
    <dc:source rdf:resource="https://github.com/scienceai/scholarly-article/issues/16"/>
    <rdf:type rdf:resource="http://www.w3.org/1999/02/22-rdf-syntax-ns#Property"/>
    <rdfs:range rdf:resource="http://schema.org/Offer"/>
  </rdf:Description>
  <rdf:Description rdf:about="http://ns.science.ai/.#Conclusion">
    <rdfs:label>Conclusion</rdfs:label>
    <owl:disjointWith rdf:resource="http://ns.science.ai/#Unspecified"/>
    <vs:term_status>testing</vs:term_status>
    <rdf:type rdf:resource="http://www.w3.org/2000/01/rdf-schema#Class"/>
    <rdfs:isDefinedBy rdf:resource="https://ns.science.ai/"/>
    <rdfs:comment>A reflection on the preceding text, summarizing the evidence, arguments or premises presented in the document and their logical outcomes. Conclusions are a fundamental feature in academic research publications, and may be included in the Discussion section.</rdfs:comment>
    <rdfs:subClassOf rdf:resource="http://purl.org/spar/deo/DiscourseElement"/>
  </rdf:Description>
  <rdf:Description rdf:about="http://ns.science.ai/.#MimeDetectionAction">
    <rdf:type rdf:resource="http://www.w3.org/2000/01/rdf-schema#Class"/>
    <rdfs:label>MimeDetectionAction</rdfs:label>
    <skos:altLabel>Mime Detection Action</skos:altLabel>
    <rdfs:comment>The act of detecting the MIME type of an object.</rdfs:comment>
    <rdfs:isDefinedBy rdf:resource="https://ns.science.ai/"/>
    <vs:term_status>testing</vs:term_status>
    <rdfs:subClassOf rdf:resource="http://schema.org/Action"/>
  </rdf:Description>
  <rdf:Description rdf:about="http://ns.science.ai/.#ImageProcessingAction">
    <rdfs:subClassOf rdf:resource="http://schema.org/Action"/>
    <skos:altLabel>Image Processing Action</skos:altLabel>
    <vs:term_status>testing</vs:term_status>
    <rdfs:comment>The act of converting an image object to web first format and extracting metadata about the object.</rdfs:comment>
    <rdf:type rdf:resource="http://www.w3.org/2000/01/rdf-schema#Class"/>
    <rdfs:label>ImageProcessingAction</rdfs:label>
    <rdfs:isDefinedBy rdf:resource="https://ns.science.ai/"/>
  </rdf:Description>
  <rdf:Description rdf:about="http://ns.science.ai/.#SupportingInformation">
    <skos:altLabel>supplementary files</skos:altLabel>
    <rdfs:isDefinedBy rdf:resource="https://ns.science.ai/"/>
    <owl:sameAs rdf:resource="http://purl.org/spar/doco/Appendix"/>
    <skos:altLabel>additional information</skos:altLabel>
    <skos:altLabel>supplementary material</skos:altLabel>
    <rdfs:label>SupportingInformation</rdfs:label>
    <vs:term_status>testing</vs:term_status>
    <skos:altLabel>supplemental material</skos:altLabel>
    <rdfs:subClassOf rdf:resource="http://purl.org/spar/deo/DiscourseElement"/>
    <skos:altLabel>additional files</skos:altLabel>
    <skos:altLabel>supplementary data</skos:altLabel>
    <rdf:type rdf:resource="http://www.w3.org/2000/01/rdf-schema#Class"/>
    <skos:altLabel>supplemental information</skos:altLabel>
    <rdfs:comment>Any information either auxiliary to the main content of the creative work or required to reproduce or verify the results of the creative work</rdfs:comment>
    <skos:altLabel>supplementary appendix</skos:altLabel>
    <skos:altLabel>additional material</skos:altLabel>
    <owl:disjointWith rdf:resource="http://ns.science.ai/#Unspecified"/>
    <skos:altLabel>appendix</skos:altLabel>
  </rdf:Description>
  <rdf:Description rdf:about="http://ns.science.ai/.#checksumAlgorithm">
    <rdfs:comment>Name of the algorithm used to compute the checksum value. Examples might include MD5, SHA-1 etc.</rdfs:comment>
    <owl:equivalentProperty rdf:resource="http://www.semanticdesktop.org/ontologies/2007/03/22/nfo/#hashAlgorithm"/>
    <rdf:type rdf:resource="http://www.w3.org/1999/02/22-rdf-syntax-ns#Property"/>
    <rdfs:isDefinedBy rdf:resource="https://ns.science.ai/"/>
    <vs:term_status>testing</vs:term_status>
    <rdfs:label>checksumAlgorithm</rdfs:label>
    <rdfs:range rdf:resource="http://www.w3.org/2001/XMLSchema#string"/>
    <rdfs:domain rdf:resource="http://ns.science.ai/#Checksum"/>
    <skos:altLabel>checksum algorithm</skos:altLabel>
    <rdfs:seeAlso rdf:resource="http://en.wikipedia.org/wiki/Checksum"/>
  </rdf:Description>
  <rdf:Description rdf:about="http://ns.science.ai/.#CsvwAction">
    <rdfs:comment>The act of extracting metadata about a tabular object compatible with the W3C Model for Tabular Data and Metadata on the Web</rdfs:comment>
    <rdfs:label>CSVWAction</rdfs:label>
    <skos:altLabel>CSVW Action</skos:altLabel>
    <rdfs:isDefinedBy rdf:resource="https://ns.science.ai/"/>
    <vs:term_status>testing</vs:term_status>
    <rdfs:subClassOf rdf:resource="http://schema.org/Action"/>
    <rdf:type rdf:resource="http://www.w3.org/2000/01/rdf-schema#Class"/>
  </rdf:Description>
  <rdf:Description rdf:about="http://ns.science.ai/.#Discussion">
    <owl:disjointWith rdf:resource="http://ns.science.ai/#Unspecified"/>
    <vs:term_status>testing</vs:term_status>
    <rdf:type rdf:resource="http://www.w3.org/2000/01/rdf-schema#Class"/>
    <rdfs:subClassOf rdf:resource="http://purl.org/spar/deo/DiscourseElement"/>
    <rdfs:comment>An interpretation and discussion of the results obtained and an analysis of their significance, in support of conclusions. These conclusions may be part of this discussion or may be included in a separate section of the document.</rdfs:comment>
    <rdfs:isDefinedBy rdf:resource="https://ns.science.ai/"/>
    <rdfs:label>Discussion</rdfs:label>
  </rdf:Description>
  <rdf:Description rdf:about="http://ns.science.ai/.#DocumentObject">
    <rdfs:comment>The most generic type for creative work encodings that are documents (HTML, LaTEX, DOCX, etc.)</rdfs:comment>
    <rdf:type rdf:resource="http://www.w3.org/2000/01/rdf-schema#Class"/>
    <rdfs:isDefinedBy rdf:resource="https://ns.science.ai/"/>
    <rdfs:label>DocumentObject</rdfs:label>
    <skos:altLabel>Document Object</skos:altLabel>
    <rdfs:subClassOf rdf:resource="http://schema.org/MediaObject"/>
    <vs:term_status>testing</vs:term_status>
  </rdf:Description>
  <rdf:Description rdf:about="http://ns.science.ai/.#SemanticTaggingAction">
    <rdfs:comment>The act of extracting semantic tags provided by web ontologies (OWL) or vocabularies (RDF Schema) from an object.</rdfs:comment>
    <rdfs:subClassOf rdf:resource="http://schema.org/Action"/>
    <rdf:type rdf:resource="http://www.w3.org/2000/01/rdf-schema#Class"/>
    <rdfs:label>SemanticTaggingAction</rdfs:label>
    <vs:term_status>testing</vs:term_status>
    <skos:altLabel>Semantic Tagging Action</skos:altLabel>
    <rdfs:isDefinedBy rdf:resource="https://ns.science.ai/"/>
  </rdf:Description>
  <rdf:Description rdf:about="http://ns.science.ai/.#Acknowledgements">
    <rdfs:label>Acknowledgements</rdfs:label>
    <rdf:type rdf:resource="http://www.w3.org/2000/01/rdf-schema#Class"/>
    <owl:sameAs rdf:resource="http://purl.org/spar/deo/Acknowledgements"/>
    <rdfs:isDefinedBy rdf:resource="https://ns.science.ai/"/>
    <rdfs:subClassOf rdf:resource="http://purl.org/spar/deo/DiscourseElement"/>
    <rdfs:comment>Usually part of the preface, or a separate section in its own right, often as part of the back matter, it acknowledges those, including funding agencies, who contributed to the undertaking of a research project described in a publication, or to the creation of the work in some way. In scientific articles, the acknowledgements are usually placed as a separated section immediately following the Discussion or Conclusions.</rdfs:comment>
    <owl:disjointWith rdf:resource="http://ns.science.ai/#Unspecified"/>
    <vs:term_status>testing</vs:term_status>
  </rdf:Description>
  <rdf:Description rdf:about="http://ns.science.ai/.#Reference">
    <vs:term_status>testing</vs:term_status>
    <skos:altLabel>Citation</skos:altLabel>
    <rdfs:label>Reference</rdfs:label>
    <rdfs:isDefinedBy rdf:resource="https://ns.science.ai/"/>
    <rdfs:comment>A reference to a specific part of the document, or to another publication.</rdfs:comment>
    <rdfs:subClassOf rdf:resource="http://purl.org/spar/deo/DiscourseElement"/>
    <owl:disjointWith rdf:resource="http://ns.science.ai/#Unspecified"/>
    <rdf:type rdf:resource="http://www.w3.org/2000/01/rdf-schema#Class"/>
    <owl:sameAs rdf:resource="http://purl.org/spar/deo/Reference"/>
  </rdf:Description>
  <rdf:Description rdf:about="http://ns.science.ai/.#MaterialsAndMethods">
    <owl:unionOf rdf:resource="http://purl.org/spar/deo/Materials"/>
    <rdf:type rdf:resource="http://www.w3.org/2000/01/rdf-schema#Class"/>
    <owl:unionOf rdf:resource="http://purl.org/spar/deo/Methods"/>
    <rdfs:label>MaterialsAndMethods</rdfs:label>
    <owl:disjointWith rdf:resource="http://ns.science.ai/#Unspecified"/>
    <skos:altLabel>Methods</skos:altLabel>
    <rdfs:isDefinedBy rdf:resource="https://ns.science.ai/"/>
    <skos:altLabel>Materials</skos:altLabel>
    <rdfs:subClassOf rdf:resource="http://purl.org/spar/deo/DiscourseElement"/>
    <vs:term_status>testing</vs:term_status>
    <skos:altLabel>Materials And Methods</skos:altLabel>
    <rdfs:comment>A description in a research paper documenting the specialized materials and/or methods used in the work described. This description is contained in a section often entitled 'Methods and Materials', 'Experimental' or a related term.</rdfs:comment>
  </rdf:Description>
  <rdf:Description rdf:about="http://ns.science.ai/.#Audio">
    <owl:disjointWith rdf:resource="http://ns.science.ai/#Unspecified"/>
    <rdfs:subClassOf rdf:resource="http://schema.org/CreativeWork"/>
    <vs:term_status>testing</vs:term_status>
    <rdf:type rdf:resource="http://www.w3.org/2000/01/rdf-schema#Class"/>
    <rdfs:label>Audio</rdfs:label>
    <rdfs:isDefinedBy rdf:resource="https://ns.science.ai/"/>
    <rdfs:comment>An audio resource</rdfs:comment>
  </rdf:Description>
  <rdf:Description rdf:about="http://ns.science.ai/.#Image">
    <rdfs:isDefinedBy rdf:resource="https://ns.science.ai/"/>
    <vs:term_status>testing</vs:term_status>
    <rdfs:subClassOf rdf:resource="http://schema.org/CreativeWork"/>
    <owl:sameAs rdf:resource="http://purl.org/spar/doco/Figure"/>
    <owl:disjointWith rdf:resource="http://ns.science.ai/#Unspecified"/>
    <rdfs:comment>An image resource</rdfs:comment>
    <rdfs:label>Image</rdfs:label>
    <rdf:type rdf:resource="http://www.w3.org/2000/01/rdf-schema#Class"/>
  </rdf:Description>
  <rdf:Description rdf:about="http://ns.science.ai/.#roleContactPoint">
    <rdfs:domain rdf:resource="http://ns.science.ai/#AuthoringRole"/>
    <rdfs:comment>A contact point for the person or organization behind an authoring role.</rdfs:comment>
    <rdfs:label>roleContactPoint</rdfs:label>
    <skos:altLabel>role contact point</skos:altLabel>
    <vs:term_status>testing</vs:term_status>
    <rdf:type rdf:resource="http://www.w3.org/1999/02/22-rdf-syntax-ns#Property"/>
    <rdfs:range rdf:resource="http://schema.org/ContactPoint"/>
    <dc:source rdf:resource="https://github.com/scienceai/scholarly.vernacular.io/issues/32"/>
    <rdfs:isDefinedBy rdf:resource="https://ns.science.ai/"/>
  </rdf:Description>
  <rdf:Description rdf:about="http://ns.science.ai/.#FormulaObject">
    <rdf:type rdf:resource="http://www.w3.org/2000/01/rdf-schema#Class"/>
    <rdfs:isDefinedBy rdf:resource="https://ns.science.ai/"/>
    <rdfs:subClassOf rdf:resource="http://purl.org/spar/deo/DiscourseElement"/>
    <skos:altLabel>Formula Object</skos:altLabel>
    <owl:sameAs rdf:resource="http://purl.org/spar/doco/FormulaBox"/>
    <rdfs:label>FormulaObject</rdfs:label>
    <vs:term_status>testing</vs:term_status>
    <rdfs:subClassOf rdf:resource="http://schema.org/MediaObject"/>
    <rdfs:comment>A formula object embedded in a web page</rdfs:comment>
  </rdf:Description>
  <rdf:Description rdf:about="http://ns.science.ai/.#DisclosureStatement">
    <rdfs:comment>A disclosure statement</rdfs:comment>
    <skos:altLabel>Disclosure Statement</skos:altLabel>
    <vs:term_status>testing</vs:term_status>
    <rdfs:isDefinedBy rdf:resource="https://ns.science.ai/"/>
    <rdfs:subClassOf rdf:resource="http://schema.org/Comment"/>
    <dc:source rdf:resource="https://github.com/scienceai/scholarly-article/issues/19"/>
    <rdf:type rdf:resource="http://www.w3.org/2000/01/rdf-schema#Class"/>
    <rdfs:label>DisclosureStatement</rdfs:label>
  </rdf:Description>
  <rdf:Description rdf:about="http://ns.science.ai/.#AudioVideoProcessingAction">
    <rdfs:label>AudioVideoProcessingAction</rdfs:label>
    <rdfs:isDefinedBy rdf:resource="https://ns.science.ai/"/>
    <vs:term_status>testing</vs:term_status>
    <rdfs:subClassOf rdf:resource="http://schema.org/Action"/>
    <skos:altLabel>Audio Video Processing Action</skos:altLabel>
    <rdf:type rdf:resource="http://www.w3.org/2000/01/rdf-schema#Class"/>
    <rdfs:comment>The act of converting an audio or video object to web first format and extracting metadata about the object.</rdfs:comment>
  </rdf:Description>
  <rdf:Description rdf:about="http://ns.science.ai/.#Authors">
    <vs:term_status>testing</vs:term_status>
    <rdfs:label>Authors</rdfs:label>
    <rdf:type rdf:resource="http://www.w3.org/2000/01/rdf-schema#Class"/>
    <rdfs:isDefinedBy rdf:resource="https://ns.science.ai/"/>
    <skos:altLabel>Author</skos:altLabel>
    <owl:disjointWith rdf:resource="http://ns.science.ai/#Unspecified"/>
    <rdfs:subClassOf rdf:resource="http://purl.org/spar/doco/ListOfAuthors"/>
    <rdfs:comment>A list of items each denoting an author of a particular publication.</rdfs:comment>
  </rdf:Description>
  <rdf:Description rdf:about="http://ns.science.ai/.#UploadAction">
    <rdfs:subClassOf rdf:resource="http://schema.org/Action"/>
    <rdfs:label>UploadAction</rdfs:label>
    <vs:term_status>testing</vs:term_status>
    <rdf:type rdf:resource="http://www.w3.org/2000/01/rdf-schema#Class"/>
    <skos:altLabel>Upload Action</skos:altLabel>
    <rdfs:comment>The act of uploading an object to an entry point within some Web-based protocol.</rdfs:comment>
    <rdfs:isDefinedBy rdf:resource="https://ns.science.ai/"/>
  </rdf:Description>
  <rdf:Description rdf:about="http://ns.science.ai/.#Introduction">
    <rdfs:comment>An initial description which states the purpose and goals of the following writing, and, in the case of journal articles, typically includes background information on the research topic and a review of related work in the area.</rdfs:comment>
    <rdfs:label>Introduction</rdfs:label>
    <rdfs:isDefinedBy rdf:resource="https://ns.science.ai/"/>
    <vs:term_status>testing</vs:term_status>
    <owl:sameAs rdf:resource="http://purl.org/spar/deo/Introduction"/>
    <rdfs:subClassOf rdf:resource="http://purl.org/spar/deo/DiscourseElement"/>
    <rdf:type rdf:resource="http://www.w3.org/2000/01/rdf-schema#Class"/>
    <owl:disjointWith rdf:resource="http://ns.science.ai/#Unspecified"/>
  </rdf:Description>
  <rdf:Description rdf:about="http://ns.science.ai/.#FundingSource">
    <rdf:type rdf:resource="http://www.w3.org/2000/01/rdf-schema#Class"/>
    <rdfs:comment>The most generic type of funding source</rdfs:comment>
    <rdfs:isDefinedBy rdf:resource="https://ns.science.ai/"/>
    <rdfs:label>FundingSource</rdfs:label>
    <dc:source rdf:resource="https://github.com/scienceai/scholarly-article/issues/16"/>
    <rdfs:subClassOf rdf:resource="http://schema.org/Offer"/>
    <vs:term_status>testing</vs:term_status>
    <skos:altLabel>Funding Source</skos:altLabel>
  </rdf:Description>
  <rdf:Description rdf:about="http://ns.science.ai/.#PerceptualHash">
    <skos:altLabel>Perceptual Hash</skos:altLabel>
    <rdfs:label>PerceptualHash</rdfs:label>
    <rdfs:comment>A fingerprint of a multimedia file derived from various features from its content. Unlike cryptographic hash functions which rely on the avalanche effect of small changes in input leading to drastic changes in the output, perceptual hashes are close to one another if the features are similar and are resiliant to transformations such as rotation, skew, contrast adjustment and different compression/formats.</rdfs:comment>
    <rdf:type rdf:resource="http://www.w3.org/2000/01/rdf-schema#Class"/>
    <skos:altLabel>pHash</skos:altLabel>
    <rdfs:seeAlso rdf:resource="https://en.wikipedia.org/wiki/Perceptual_hashing"/>
    <rdfs:subClassOf rdf:resource="http://ns.science.ai/#Checksum"/>
    <rdfs:isDefinedBy rdf:resource="https://ns.science.ai/"/>
    <vs:term_status>testing</vs:term_status>
  </rdf:Description>
  <rdf:Description rdf:about="http://ns.science.ai/.#TableObject">
    <rdfs:comment>A table object embedded in a web page</rdfs:comment>
    <skos:altLabel>Table Object</skos:altLabel>
    <rdfs:subClassOf rdf:resource="http://schema.org/MediaObject"/>
    <rdfs:isDefinedBy rdf:resource="https://ns.science.ai/"/>
    <owl:sameAs rdf:resource="http://purl.org/spar/doco/TableBox"/>
    <rdfs:label>TableObject</rdfs:label>
    <vs:term_status>testing</vs:term_status>
    <rdf:type rdf:resource="http://www.w3.org/2000/01/rdf-schema#Class"/>
  </rdf:Description>
  <rdf:Description rdf:about="http://ns.science.ai/.#Results">
    <rdfs:subClassOf rdf:resource="http://purl.org/spar/deo/DiscourseElement"/>
    <rdfs:comment>The report of the specific findings of an investigation, given without discussion or conclusion being drawn.</rdfs:comment>
    <owl:sameAs rdf:resource="http://purl.org/spar/deo/Results"/>
    <owl:disjointWith rdf:resource="http://ns.science.ai/#Unspecified"/>
    <rdf:type rdf:resource="http://www.w3.org/2000/01/rdf-schema#Class"/>
    <rdfs:isDefinedBy rdf:resource="https://ns.science.ai/"/>
    <vs:term_status>testing</vs:term_status>
    <rdfs:label>Results</rdfs:label>
  </rdf:Description>
  <rdf:Description rdf:about="http://ns.science.ai/.#Video">
    <rdfs:subClassOf rdf:resource="http://schema.org/CreativeWork"/>
    <rdf:type rdf:resource="http://www.w3.org/2000/01/rdf-schema#Class"/>
    <rdfs:comment>A video resource</rdfs:comment>
    <rdfs:label>Video</rdfs:label>
    <rdfs:isDefinedBy rdf:resource="https://ns.science.ai/"/>
    <vs:term_status>testing</vs:term_status>
    <owl:disjointWith rdf:resource="http://ns.science.ai/#Unspecified"/>
  </rdf:Description>
  <rdf:Description rdf:about="http://ns.science.ai/.#Checksum">
    <vs:term_status>testing</vs:term_status>
    <rdfs:label>Checksum</rdfs:label>
    <rdfs:comment>A small-size datum from an arbitrary block of digital data for the purpose of detecting errors which may have been introduced during its transmission or storage.</rdfs:comment>
    <rdfs:isDefinedBy rdf:resource="https://ns.science.ai/"/>
    <rdfs:seeAlso rdf:resource="http://en.wikipedia.org/wiki/Checksum"/>
    <rdfs:subClassOf rdf:resource="http://schema.org/Intangible"/>
    <rdf:type rdf:resource="http://www.w3.org/2000/01/rdf-schema#Class"/>
  </rdf:Description>
  <rdf:Description rdf:about="http://ns.science.ai/.#ReferenceList">
    <skos:altLabel>Citations</skos:altLabel>
    <skos:altLabel>References</skos:altLabel>
    <owl:sameAs rdf:resource="http://purl.org/spar/doco/ListOfReferences"/>
    <vs:term_status>testing</vs:term_status>
    <skos:altLabel>Bibliography</skos:altLabel>
    <rdfs:label>ReferenceList</rdfs:label>
    <rdf:type rdf:resource="http://www.w3.org/2000/01/rdf-schema#Class"/>
    <rdfs:isDefinedBy rdf:resource="https://ns.science.ai/"/>
    <skos:altLabel>Works Cited</skos:altLabel>
    <rdfs:comment>A list of items each representing a reference to a specific part of the same document, or to another publication.</rdfs:comment>
    <skos:altLabel>Literature</skos:altLabel>
    <owl:disjointWith rdf:resource="http://ns.science.ai/#Unspecified"/>
    <rdfs:subClassOf rdf:resource="http://purl.org/spar/doco/List"/>
  </rdf:Description>
  <rdf:Description rdf:about="http://ns.science.ai/.#Formula">
    <owl:disjointWith rdf:resource="http://ns.science.ai/#Unspecified"/>
    <rdfs:label>Formula</rdfs:label>
    <rdfs:subClassOf rdf:resource="http://purl.org/spar/deo/DiscourseElement"/>
    <rdfs:comment>A unit of information expressed in mathematical, chemical or logical symbols and language.</rdfs:comment>
    <vs:term_status>testing</vs:term_status>
    <owl:sameAs rdf:resource="http://purl.org/spar/doco/Formula"/>
    <skos:altLabel>Equation</skos:altLabel>
    <rdfs:subClassOf rdf:resource="http://schema.org/CreativeWork"/>
    <rdfs:isDefinedBy rdf:resource="https://ns.science.ai/"/>
    <rdf:type rdf:resource="http://www.w3.org/2000/01/rdf-schema#Class"/>
  </rdf:Description>
  <rdf:Description rdf:about="http://ns.science.ai/.#contentChecksum">
    <vs:term_status>testing</vs:term_status>
    <rdfs:range rdf:resource="http://ns.science.ai/#Checksum"/>
    <rdfs:domain rdf:resource="http://schema.org/CreativeWork"/>
    <rdfs:comment>The checksum of a resource.</rdfs:comment>
    <rdfs:isDefinedBy rdf:resource="https://ns.science.ai/"/>
    <owl:equivalentProperty rdf:resource="http://www.semanticdesktop.org/ontologies/2007/03/22/nfo/#hasHash"/>
    <rdf:type rdf:resource="http://www.w3.org/1999/02/22-rdf-syntax-ns#Property"/>
    <rdfs:seeAlso rdf:resource="http://en.wikipedia.org/wiki/Checksum"/>
    <skos:altLabel>content checksum</skos:altLabel>
    <rdfs:label>contentChecksum</rdfs:label>
  </rdf:Description>
  <rdf:Description rdf:about="http://ns.science.ai/.#AcknowledgementStatement">
    <rdfs:comment>An acknowledgement statement</rdfs:comment>
    <vs:term_status>testing</vs:term_status>
    <rdf:type rdf:resource="http://www.w3.org/2000/01/rdf-schema#Class"/>
    <rdfs:isDefinedBy rdf:resource="https://ns.science.ai/"/>
    <rdfs:subClassOf rdf:resource="http://schema.org/Comment"/>
    <dc:source rdf:resource="https://github.com/scienceai/scholarly-article/issues/19"/>
    <skos:altLabel>Acknowledgement Statement</skos:altLabel>
    <rdfs:label>AcknowledgementStatement</rdfs:label>
  </rdf:Description>
  <rdf:Description rdf:about="http://ns.science.ai/.#Abstract">
    <rdfs:subClassOf rdf:resource="http://schema.org/CreativeWork"/>
    <rdf:type rdf:resource="http://www.w3.org/2000/01/rdf-schema#Class"/>
    <rdfs:label>Abstract</rdfs:label>
    <vs:term_status>testing</vs:term_status>
    <rdfs:isDefinedBy rdf:resource="https://ns.science.ai/"/>
    <rdfs:comment>A brief summary of a book, a research article, thesis, review, conference proceeding or any in-depth analysis of a particular subject or discipline, the purpose of which is to help the reader quickly ascertain the publication's purpose.</rdfs:comment>
    <owl:disjointWith rdf:resource="http://ns.science.ai/#Unspecified"/>
  </rdf:Description>
  <rdf:Description rdf:about="http://ns.science.ai/.#roleAffiliation">
    <rdfs:domain rdf:resource="http://ns.science.ai/#AuthoringRole"/>
    <rdfs:label>roleAffiliation</rdfs:label>
    <skos:altLabel>role affiliation</skos:altLabel>
    <dc:source rdf:resource="https://github.com/scienceai/scholarly.vernacular.io/issues/32"/>
    <rdfs:isDefinedBy rdf:resource="https://ns.science.ai/"/>
    <vs:term_status>testing</vs:term_status>
    <rdf:type rdf:resource="http://www.w3.org/1999/02/22-rdf-syntax-ns#Property"/>
    <rdfs:range rdf:resource="http://schema.org/Organization"/>
    <rdfs:comment>The affiliation under which the role was performed.</rdfs:comment>
  </rdf:Description>
  <rdf:Description rdf:about="http://ns.science.ai/.#roleComment">
    <dc:source rdf:resource="https://github.com/scienceai/scholarly-article/issues/19"/>
    <rdf:type rdf:resource="http://www.w3.org/1999/02/22-rdf-syntax-ns#Property"/>
    <rdfs:comment>role comments such as author notes, disclosure statements or acknowledgement statements</rdfs:comment>
    <rdfs:isDefinedBy rdf:resource="https://ns.science.ai/"/>
    <rdfs:domain rdf:resource="http://ns.science.ai/#ContributorRole"/>
    <vs:term_status>testing</vs:term_status>
    <skos:altLabel>role comment</skos:altLabel>
    <rdfs:range rdf:resource="http://schema.org/Comment"/>
    <rdfs:label>roleComment</rdfs:label>
  </rdf:Description>
  <rdf:Description rdf:about="http://ns.science.ai/.#Funding">
    <rdf:type rdf:resource="http://www.w3.org/2000/01/rdf-schema#Class"/>
    <rdfs:isDefinedBy rdf:resource="https://ns.science.ai/"/>
    <vs:term_status>testing</vs:term_status>
    <rdfs:subClassOf rdf:resource="http://purl.org/spar/deo/DiscourseElement"/>
    <owl:disjointWith rdf:resource="http://ns.science.ai/#Unspecified"/>
    <rdfs:label>Funding</rdfs:label>
    <rdfs:comment>Person or Organization that funded the research on which a work was based.</rdfs:comment>
  </rdf:Description>
  <rdf:Description rdf:about="http://ns.science.ai/.#Disclosure">
    <skos:altLabel>Competing Interest</skos:altLabel>
    <owl:disjointWith rdf:resource="http://ns.science.ai/#Unspecified"/>
    <rdfs:subClassOf rdf:resource="http://schema.org/CreativeWork"/>
    <skos:altLabel>Conflict of Interest</skos:altLabel>
    <rdf:type rdf:resource="http://www.w3.org/2000/01/rdf-schema#Class"/>
    <rdfs:isDefinedBy rdf:resource="https://ns.science.ai/"/>
    <rdfs:comment>A section containing acknowledgment of facts that interfere with or could reasonably be perceived as interfering with the full and objective presentation, peer review, editorial decision-making, or publication of research</rdfs:comment>
    <vs:term_status>testing</vs:term_status>
    <rdfs:label>Disclosure</rdfs:label>
  </rdf:Description>
  <rdf:Description rdf:about="http://ns.science.ai/.#checksumValue">
    <rdfs:domain rdf:resource="http://ns.science.ai/#Checksum"/>
    <rdfs:seeAlso rdf:resource="http://en.wikipedia.org/wiki/Checksum"/>
    <rdfs:range rdf:resource="http://www.w3.org/2001/XMLSchema#string"/>
    <rdfs:label>checksumValue</rdfs:label>
    <owl:equivalentProperty rdf:resource="http://www.semanticdesktop.org/ontologies/2007/03/22/nfo/#hashValue"/>
    <rdfs:comment>The actual value of the hash in base64 if no datatype are present.</rdfs:comment>
    <rdfs:isDefinedBy rdf:resource="https://ns.science.ai/"/>
    <vs:term_status>testing</vs:term_status>
    <skos:altLabel>checksum</skos:altLabel>
    <rdf:type rdf:resource="http://www.w3.org/1999/02/22-rdf-syntax-ns#Property"/>
    <skos:altLabel>hash</skos:altLabel>
  </rdf:Description>
  <rdf:Description rdf:about="http://ns.science.ai/.#SponsorRole">
    <rdf:type rdf:resource="http://www.w3.org/2000/01/rdf-schema#Class"/>
    <rdfs:subClassOf rdf:resource="http://schema.org/Role"/>
    <rdfs:isDefinedBy rdf:resource="https://ns.science.ai/"/>
    <rdfs:label>SponsorRole</rdfs:label>
    <dc:source rdf:resource="https://github.com/scienceai/scholarly-article/issues/16"/>
    <rdfs:comment>A subclass of Role used to describe sponsoring roles.</rdfs:comment>
    <vs:term_status>testing</vs:term_status>
    <skos:altLabel>Sponsor Role</skos:altLabel>
  </rdf:Description>
  <rdf:Description rdf:about="http://ns.science.ai/.#Affiliations">
    <skos:altLabel>Affiliation</skos:altLabel>
    <rdfs:label>Affiliations</rdfs:label>
    <owl:disjointWith rdf:resource="http://ns.science.ai/#Unspecified"/>
    <rdfs:comment>A list of affiliations for the authors and contributors.</rdfs:comment>
    <rdfs:subClassOf rdf:resource="http://purl.org/spar/doco/ListOfOrganizations"/>
    <rdfs:isDefinedBy rdf:resource="https://ns.science.ai/"/>
    <vs:term_status>testing</vs:term_status>
    <rdf:type rdf:resource="http://www.w3.org/2000/01/rdf-schema#Class"/>
  </rdf:Description>
  <rdf:Description rdf:about="http://ns.science.ai/.#ContributorRole">
    <rdfs:comment>A subclass of Role used to describe contributor roles.</rdfs:comment>
    <rdf:type rdf:resource="http://www.w3.org/2000/01/rdf-schema#Class"/>
    <skos:altLabel>Contributor Role</skos:altLabel>
    <rdfs:label>ContributorRole</rdfs:label>
    <dc:source rdf:resource="https://github.com/scienceai/scholarly.vernacular.io/issues/32"/>
    <vs:term_status>testing</vs:term_status>
    <rdfs:subClassOf rdf:resource="http://schema.org/Role"/>
    <rdfs:isDefinedBy rdf:resource="https://ns.science.ai/"/>
  </rdf:Description>
  <rdf:Description rdf:about="http://ns.science.ai/.#Contributors">
    <vs:term_status>testing</vs:term_status>
    <rdfs:label>Contributors</rdfs:label>
    <rdfs:comment>A list of items, each denoting a contributor to a publication where such contributions are insufficient to warrant classification as author.</rdfs:comment>
    <rdfs:isDefinedBy rdf:resource="https://ns.science.ai/"/>
    <rdf:type rdf:resource="http://www.w3.org/2000/01/rdf-schema#Class"/>
    <owl:disjointWith rdf:resource="http://ns.science.ai/#Unspecified"/>
    <skos:altLabel>Contributor</skos:altLabel>
    <rdfs:subClassOf rdf:resource="http://purl.org/spar/doco/ListOfContributors"/>
  </rdf:Description>
  <rdf:Description rdf:about="http://ns.science.ai/.#doi">
    <rdfs:domain rdf:resource="http://schema.org/CreativeWork"/>
    <rdf:type rdf:resource="http://www.w3.org/1999/02/22-rdf-syntax-ns#Property"/>
    <rdfs:label>doi</rdfs:label>
    <rdfs:isDefinedBy rdf:resource="https://ns.science.ai/"/>
    <vs:term_status>testing</vs:term_status>
    <rdfs:range rdf:resource="http://schema.org/URL"/>
    <rdfs:comment>A digital object identifier (DOI) for the resource.</rdfs:comment>
    <rdfs:seeAlso rdf:resource="https://en.wikipedia.org/wiki/Digital_object_identifier"/>
    <owl:equivalentProperty rdf:resource="http://purl.org/ontology/bibo/doi"/>
  </rdf:Description>
</rdf:RDF>

